theories/Optim.v
@@ -3,8 +3,8 @@ From Coq Require Import Bool String List BinPos Compare_dec Omega.
 From Equations Require Import Equations DepElimDec.
 From Template Require Import Ast utils Typing.
 From Translation
-Require Import util Sorts SAst SLiftSubst Equality SCommon XTyping Conversion
-ITyping ITypingInversions ITypingLemmata ITypingAdmissible DecideConversion.
+Require Import util Sorts SAst SLiftSubst Equality SCommon XTyping
+ITyping ITypingInversions ITypingLemmata ITypingAdmissible.
 
 Section Optim.
 
