theories/SAst.v
@@ -23,6 +23,7 @@ Inductive sterm : Type :=
 | sRefl (A u : sterm)
 | sJ (A u P w v p : sterm)
 | sTransport (T1 T2 p t : sterm)
+| sBeta (f t : sterm)
 (* Heterogenous equality *)
 | sHeq (A a B b : sterm)
 | sHeqToEq (p : sterm)
